new/proof/github_com/goose_lang/goose/model/channel/protocol/done/done.v
@@ -19,7 +19,7 @@ From iris.base_logic.lib Require Import saved_prop.
 
 Section done.
 Context `{hG: heapGS Σ, !ffi_semantics _ _}.
-Context `{!chanGhostStateG Σ V}.
+Context `{!chanG Σ V}.
 Context `{!IntoVal V}.
 Context `{!IntoValTyped V t}.
 Context `{!globalsGS Σ} {go_ctx : GoContext}.
