new/proof/github_com/goose_lang/goose/model/channel/protocol/join/join.v
@@ -35,7 +35,7 @@ Proof. solve_inG. Qed.
 
 Section proof.
 Context `{hG: heapGS Σ, !ffi_semantics _ _}.
-Context `{!chanGhostStateG Σ V}.
+Context `{!chanG Σ V}.
 Context `{!IntoVal V}.
 Context `{!IntoValTyped V t}.
 Context `{!globalsGS Σ} {go_ctx : GoContext}.
