new/proof/github_com/goose_lang/goose/testdata/examples/channel_search_replace.v
@@ -9,7 +9,7 @@ Section proof.
 Context `{hG: heapGS Σ, !ffi_semantics _ _}.
 Context `{!globalsGS Σ} {go_ctx : GoContext}.
 Context `{!syncG Σ}.
-Context `{!chanGhostStateG Σ slice.t}.
+Context `{!chanG Σ slice.t}.
 Context `{!waitgroup_joinG Σ}.
 
 #[global] Instance : IsPkgInit chan_spec_raw_examples := define_is_pkg_init True%I.
@@ -113,7 +113,7 @@ Lemma wp_SearchReplace (s: slice.t) (xs: list w64) (x y: w64) :
   }}}
     @! chan_spec_raw_examples.SearchReplace #s #x #y
   {{{ RET #(); s ↦* (search_replace x y xs) }}}.
-Proof using chanGhostStateG0 waitgroup_joinG0 syncG0.
+Proof using chanG0 waitgroup_joinG0 syncG0.
   (* The first overflow:
      implementation adds 1000 at a time, potentially surpassing the slice length
      before clamping. If it goes negative, then the clamping doesn't work. This
